VLSM/Equivocators/Composition/Common.v
@@ -1,0 +1,1007 @@
+Require Import
+  List Coq.Vectors.Fin FinFun
+  Arith.Compare_dec Lia
+  Program
+  Coq.Logic.JMeq
+  .
+Import ListNotations.
+From CasperCBC
+  Require Import
+    Preamble ListExtras FinExtras FinFunExtras
+    VLSM.Common VLSM.Composition VLSM.Equivocation
+    VLSM.Equivocators.Common VLSM.Equivocators.Projections
+    VLSM.Equivocators.MessageProperties
+    .
+
+(** ** Equivocator composition
+
+Given a composition <<X>> of VLSMs, we can model equivocator behavior by
+creating an _equivocator composition_ which replaces each component of <<X>>
+with its equivocator version and strengthens the composition constraint to
+allow no (additional) equivocations, that is, all messages being received
+must have been previously sent by one of the (equivocator) VLSMs in the
+composition.
+*)
+
+(** ** Extracting equivocator traces from equivocator composition traces
+To recover the equivocator trace for the regular composition <<X>> from
+the traces of the equivocator composition, we'll assume that only the
+first state copy of each machine is observable in the composition
+and we ignore the activity corresponding to any other state copy,
+including the forks.
+
+This amounts to removing from the trace all transitions in which the
+state copy index is not 1, forgetting the additional components of
+the label, and keeping only the copy of index 1 for each machine.
+
+*)
+
+Section fully_equivocating_composition.
+
+Context {message : Type}
+  {equiv_index nequiv_index : Type}
+  (index := sum equiv_index nequiv_index)
+  {IndEqDec : EqDecision index}
+  (IM : index -> VLSM message)
+  (Hbs : forall i : index, has_been_sent_capability (IM i))
+  (i0 : index)
+  (X := free_composite_vlsm IM i0)
+  .
+
+Local Instance equiv_index_eq_dec : EqDecision equiv_index.
+Proof.
+  intros x y.
+  destruct (decide (inl x = inl y)).
+  - left. inversion e. reflexivity.
+  - right. intro contra. elim n. subst. reflexivity.
+Qed.
+
+Definition equivocator_IM
+  (i : index)
+  : VLSM message
+  :=
+  match i with
+  | inl _ => equivocator_vlsm (IM i)
+  | inr _ => (IM i)
+  end.
+
+Lemma equivocator_Hbs
+  (i : index)
+  :  has_been_sent_capability (equivocator_IM i).
+Proof.
+  unfold equivocator_IM.
+  destruct i as [eqv | neqv] eqn:Hi.
+  - apply equivocator_has_been_sent_capability. apply Hbs.
+  - apply Hbs.
+Qed.
+
+Context
+  (index_listing : list index)
+  (finite_index : Listing index_listing)
+  (equiv_listing := left_listing finite_index)
+  (finite_equiv := left_finite finite_index)
+  .
+
+Definition equivocators_no_equivocations_constraint
+  (l : composite_label equivocator_IM)
+  (som : composite_state equivocator_IM * option message)
+  : Prop
+  :=
+  no_equivocations equivocator_IM i0 (free_constraint equivocator_IM) finite_index equivocator_Hbs l som.
+
+Definition equivocators_constrained_vlsm
+  (constraint :  composite_label equivocator_IM -> composite_state equivocator_IM * option message -> Prop)
+  : VLSM message
+  :=
+  composite_vlsm equivocator_IM i0 constraint.
+
+Let equivocators_free_vlsm := equivocators_constrained_vlsm (free_constraint equivocator_IM).
+
+Definition equivocators_no_equivocations_vlsm
+  : VLSM message
+  :=
+  equivocators_constrained_vlsm equivocators_no_equivocations_constraint.
+
+Lemma equivocators_initial_state_size
+  (is : vstate equivocators_no_equivocations_vlsm)
+  (His : vinitial_state_prop equivocators_no_equivocations_vlsm is)
+  (eqv : equiv_index)
+  : projT1 (is (inl eqv)) = 0.
+Proof.
+  specialize (His (inl eqv)).
+  destruct His as [Hzero His].
+  assumption.
+Qed.
+
+Definition equivocators_choice : Type := forall (eqv : equiv_index), MachineDescriptor (IM (inl eqv)).
+
+Definition proper_equivocators_choice
+  (eqv_choice : equivocators_choice)
+  (s : vstate equivocators_free_vlsm)
+  : Prop
+  := forall
+    (eqv : equiv_index),
+    proper_descriptor (IM (inl eqv)) (eqv_choice eqv) (s (inl eqv)).
+
+Definition not_equivocating_equivocators_choice
+  (eqv_choice : equivocators_choice)
+  (s : vstate equivocators_free_vlsm)
+  : Prop
+  := forall
+    (eqv : equiv_index),
+    not_equivocating_descriptor (IM (inl eqv)) (eqv_choice eqv) (s (inl eqv)).
+
+Lemma not_equivocating_equivocators_choice_proper
+  (eqv_choice : equivocators_choice)
+  (s : vstate equivocators_free_vlsm)
+  (Hne : not_equivocating_equivocators_choice eqv_choice s)
+  : proper_equivocators_choice eqv_choice s.
+Proof.
+  intro eqv. apply not_equivocating_descriptor_proper. apply Hne.
+Qed.
+
+Definition zero_choice
+  (eqv : equiv_index)
+  : MachineDescriptor (IM (inl eqv))
+  := Existing _ 0 false.
+
+Lemma zero_choice_not_equivocating
+  (s : vstate equivocators_free_vlsm)
+  : not_equivocating_equivocators_choice zero_choice s.
+Proof.
+  intro eqv. simpl. lia.
+Qed.
+
+Lemma zero_choice_proper
+  (s : vstate equivocators_free_vlsm)
+  : proper_equivocators_choice zero_choice s.
+Proof.
+  apply not_equivocating_equivocators_choice_proper. apply zero_choice_not_equivocating.
+Qed.
+
+Lemma proper_equivocators_choice_state_update_eqv
+  (eqv_choice : equivocators_choice)
+  (s : vstate equivocators_free_vlsm)
+  (eqv : equiv_index)
+  (si : vstate (equivocator_IM (inl eqv)))
+  (Hsi_proper : proper_descriptor (IM (inl eqv)) (eqv_choice eqv) (s (inl eqv)))
+  (Hproper : proper_equivocators_choice eqv_choice (state_update equivocator_IM s (inl eqv) si))
+  : proper_equivocators_choice eqv_choice s.
+Proof.
+  intro eqv'.
+  specialize (Hproper eqv').
+  destruct (decide (inl eqv' = inl eqv)).
+  - inversion e. subst. rewrite state_update_eq in Hproper. assumption.
+  - rewrite state_update_neq in Hproper; assumption.
+Qed.
+
+Lemma proper_equivocators_choice_state_update_neqv
+  (eqv_choice : equivocators_choice)
+  (s : vstate equivocators_free_vlsm)
+  (neqv : nequiv_index)
+  (si : vstate (equivocator_IM (inr neqv)))
+  (Hproper : proper_equivocators_choice eqv_choice (state_update equivocator_IM s (inr neqv) si))
+  : proper_equivocators_choice eqv_choice s.
+Proof.
+  intro eqv.
+  specialize (Hproper eqv).
+  destruct (decide (inl eqv = inr neqv)); try discriminate e.
+  rewrite state_update_neq in Hproper; assumption.
+Qed.
+
+Definition equivocators_state_project
+  (eqv_choice : equivocators_choice)
+  (s : vstate equivocators_free_vlsm)
+  (i : index)
+  : vstate (IM i)
+  :=
+  let si := s i in
+  match i with
+  | inl eqv =>
+    match (eqv_choice eqv) with
+    | NewMachine _ sn => sn
+    | Existing _ j _ =>
+      let (n, bs) := s (inl eqv) in
+      match (le_lt_dec (S n) j) with
+      | right lt_in => bs (of_nat_lt lt_in)
+      | left _ => bs F1
+      end
+    end
+  | inr neqv => s (inr neqv)
+  end.
+
+Definition lift_to_equivocators_state
+  (s : vstate X)
+  (i : index)
+  : vstate (equivocator_IM i)
+  :=
+  match i with
+  | inl eqv => mk_singleton_state _ (s (inl eqv))
+  | inr neqv => s (inr neqv)
+  end.
+
+Lemma lift_initial_to_equivocators_state
+  (s : vstate X)
+  (Hs : vinitial_state_prop X s)
+  : vinitial_state_prop equivocators_no_equivocations_vlsm (lift_to_equivocators_state s).
+Proof.
+  unfold vinitial_state_prop in *. simpl in *.
+  unfold composite_initial_state_prop in *.
+  intro i. spec Hs i.
+  destruct i as [eqv | neqv].
+  - split; try assumption. reflexivity.
+  - assumption.
+Qed.
+
+(**
+A very useful operation on [equivocators_choice]s is updating the state corresponding
+to a component:
+*)
+Definition equivocators_choice_update
+  (s : equivocators_choice)
+  (i : equiv_index)
+  (si : MachineDescriptor (IM (inl i)))
+  (j : equiv_index)
+  : MachineDescriptor (IM (inl j))
+  :=
+  match decide (j = i) with
+  | left e => eq_rect_r (fun i => MachineDescriptor (IM (inl i))) si e
+  | _ => s j
+  end.
+
+(**
+The next few results describe several properties of the [equivocators_choice_update] operation.
+*)
+Lemma equivocators_choice_update_neq
+  (s : equivocators_choice)
+  (i : equiv_index)
+  (si : MachineDescriptor (IM (inl i)))
+  (j : equiv_index)
+  (Hneq : j <> i)
+  : equivocators_choice_update s i si j = s j.
+Proof.
+  unfold equivocators_choice_update. destruct (decide (j = i)); try contradiction. reflexivity.
+Qed.
+
+Lemma equivocators_choice_update_eq
+  (s : equivocators_choice)
+  (i : equiv_index)
+  (si : MachineDescriptor (IM (inl i)))
+  : equivocators_choice_update s i si i = si.
+Proof.
+  unfold equivocators_choice_update.
+  rewrite eq_dec_refl. reflexivity.
+Qed.
+
+Lemma equivocators_choice_update_id
+  (s : equivocators_choice)
+  (i : equiv_index)
+  (si : MachineDescriptor (IM (inl i)))
+  (Heq : s i = si)
+  : equivocators_choice_update s i si = s.
+Proof.
+  apply functional_extensionality_dep_good.
+  intro j.
+  destruct (decide (j = i)).
+  - subst. apply equivocators_choice_update_eq.
+  - apply equivocators_choice_update_neq. assumption.
+Qed.
+
+Lemma equivocators_choice_update_twice
+  (s : equivocators_choice)
+  (i : equiv_index)
+  (si si': MachineDescriptor (IM (inl i)))
+  : equivocators_choice_update (equivocators_choice_update s i si) i si'
+  = equivocators_choice_update s i si'.
+Proof.
+  apply functional_extensionality_dep_good.
+  intro j.
+  destruct (decide (j = i)).
+  - subst. rewrite equivocators_choice_update_eq. symmetry. apply equivocators_choice_update_eq.
+  - repeat rewrite equivocators_choice_update_neq; try assumption.
+    reflexivity.
+Qed.
+
+Lemma equivocators_state_project_state_update_neqv
+  (eqv_choice : equivocators_choice)
+  (s : vstate equivocators_free_vlsm)
+  (neqv : nequiv_index)
+  (sneqv : vstate (equivocator_IM (inr neqv)))
+  : equivocators_state_project eqv_choice (state_update equivocator_IM s (inr neqv) sneqv)
+  = state_update IM (equivocators_state_project eqv_choice s) (inr neqv) sneqv.
+Proof.
+  apply functional_extensionality_dep.
+  intro i.
+  unfold equivocators_state_project.
+  unfold state_update.
+  destruct i as [ieqv|ineqv]
+  ; match goal with
+    |- context [decide ?d] => destruct (decide d)
+    end; [discriminate e|reflexivity|..|reflexivity].
+  inversion e. subst.
+  unfold eq_rect_r.
+  elim_eq_rect.
+  reflexivity.
+Qed.
+
+Lemma equivocators_state_project_state_update_eqv
+  (eqv_choice : equivocators_choice)
+  (s : vstate equivocators_free_vlsm)
+  (eqv : equiv_index)
+  (seqv : vstate (equivocator_IM (inl eqv)))
+  : let si :=  match eqv_choice eqv with
+    | NewMachine _ sn => sn
+    | Existing _ i _ =>
+      match le_lt_dec (S (projT1 seqv)) i with
+      | left _ => projT2 seqv F1
+      | right l => projT2 seqv (of_nat_lt l)
+      end
+    end in
+  equivocators_state_project eqv_choice (state_update equivocator_IM s (inl eqv) seqv)
+  = state_update IM (equivocators_state_project eqv_choice s) (inl eqv) si.
+Proof.
+  apply functional_extensionality_dep.
+  intro i.
+  unfold equivocators_state_project.
+  unfold state_update.
+  destruct i as [ieqv|ineqv]
+  ; match goal with
+    |- context [decide ?d] => destruct (decide d)
+    end; [|reflexivity|discriminate e|reflexivity].
+  inversion e. subst. unfold eq_rect_r.
+  elim_eq_rect. unfold eq_rect.
+  destruct seqv as (n, bs).
+  reflexivity.
+Qed.
+
+Lemma equivocators_initial_state_project
+  (es : vstate equivocators_free_vlsm)
+  (Hes : vinitial_state_prop equivocators_free_vlsm es)
+  (eqv_choice : equivocators_choice)
+  (Heqv : proper_equivocators_choice eqv_choice es)
+  : vinitial_state_prop X (equivocators_state_project eqv_choice es).
+Proof.
+  intro n. specialize (Hes n).
+  unfold equivocator_IM in Hes.
+  unfold equivocators_state_project.
+  destruct n as [eqv|neqv]; try assumption.
+  specialize (Heqv eqv).
+  destruct (eqv_choice eqv) as [sn | i fi]; try assumption.
+  destruct Hes as [Hzero Hes].
+  destruct (es (inl eqv)) as (n, bs). simpl in Heqv.
+  destruct (le_lt_dec (S n) i). { lia. }
+  simpl in *.
+  subst. assert (Hi: i = 0) by lia. subst.
+  assumption.
+Qed.
+
+Lemma equivocators_initial_message
+  (m : message)
+  (Hem : vinitial_message_prop equivocators_free_vlsm m)
+  : vinitial_message_prop X m.
+Proof.
+  destruct Hem as [i [emi Hem]].
+  exists i.
+  unfold equivocator_IM in emi.
+  destruct i as [eqv | neqv]; exists emi; assumption.
+Qed.
+
+Local Tactic Notation "unfold_transition"  hyp(H) :=
+  ( unfold transition in H; unfold equivocator_vlsm in H
+  ; unfold Common.equivocator_vlsm in H
+  ; unfold mk_vlsm in H; unfold machine in H
+  ; unfold projT2 in H; unfold equivocator_vlsm_machine in H
+  ; unfold equivocator_transition in H).
+
+Lemma equivocators_protocol_state_project
+  (es : vstate equivocators_no_equivocations_vlsm)
+  (om : option message)
+  (Hes : protocol_prop equivocators_no_equivocations_vlsm (es, om))
+  : option_protocol_message_prop X om
+  /\ forall
+    (eqv_choice : equivocators_choice)
+    (Heqv : proper_equivocators_choice eqv_choice es),
+    protocol_state_prop X (equivocators_state_project eqv_choice es).
+Proof.
+  generalize_eqs Hes. intro Heq; subst.
+  revert om. revert es.
+  induction Hes; simplify_dep_elim.
+  - split.
+    + exists (proj1_sig (vs0 X)). apply (protocol_initial_state X).
+    + destruct is as [is His]. unfold s. simpl.
+      intros.
+      specialize (equivocators_initial_state_project _ His eqv_choice Heqv) as HisX.
+      remember (equivocators_state_project eqv_choice is) as isX.
+      replace isX with (proj1_sig (exist _ _ HisX)); try reflexivity.
+      exists None.
+      apply protocol_initial_state.
+  - split.
+    + exists (proj1_sig (vs0 X)). unfold om0. clear om0.
+      destruct im as [im Him]. simpl.
+      apply equivocators_initial_message in Him.
+      apply (protocol_initial_message X (exist _ im Him)).
+    + destruct s0 as [is His]. unfold s. simpl. clear s.
+      intros.
+      specialize (equivocators_initial_state_project _ His eqv_choice Heqv) as HisX.
+      remember (equivocators_state_project eqv_choice is) as isX.
+      replace isX with (proj1_sig (exist _ _ HisX)); try reflexivity.
+      exists None.
+      apply protocol_initial_state.
+  - specialize (IHHes1 s _om JMeq_refl). apply proj2 in IHHes1.
+    specialize (IHHes2 _s om0 JMeq_refl). apply proj1 in IHHes2.
+    simpl in x.
+    destruct l as (i, li).
+    destruct (vtransition (equivocator_IM i) li (s i, om0)) as (si', om') eqn:Ht.
+    inversion x. subst es om. clear x.
+    destruct Hv as [Hv _]. simpl in Hv.
+    specialize (protocol_generated X) as Hgen.
+    destruct i as [ieqv | ineqv].
+    * destruct li as (li, di).
+      specialize (Hgen (existT _ (inl ieqv) li)) as Hgen_om'.
+      simpl in Hv. unfold vvalid in Hv. simpl in Hv.
+      simpl in Ht. unfold vtransition in Ht. unfold_transition Ht.
+      unfold snd in Ht.
+      destruct di as [sn | i fi].
+      -- destruct Hv as [Hsn Hv].
+        subst om0.
+        inversion Ht. subst. clear Ht.
+        split; try assumption.
+        intros eqv_choice Heqv.
+        destruct (s (inl ieqv)) as (n, bs) eqn:Hsieqv.
+        destruct (eqv_choice ieqv) as [sieqv | iieqv fieqv] eqn:Hieqv.
+        ++ assert (Heqvs : proper_equivocators_choice eqv_choice s).
+          { intro eqv'. specialize (Heqv eqv').
+            simpl in *.
+            destruct (decide (inl eqv' = inl ieqv))
+            ; try (rewrite state_update_neq in Heqv; assumption).
+            inversion e. subst. rewrite state_update_eq in Heqv.
+            rewrite Hieqv in *. simpl in Heqv. assumption.
+          }
+          specialize (IHHes1 _ Heqvs).
+          replace
+            (equivocators_state_project eqv_choice
+            (state_update equivocator_IM s (inl ieqv)
+               (equivocator_state_extend (IM (inl ieqv))
+                  (existT (fun n0 : nat => t (S n0) -> vstate (IM (inl ieqv))) n bs)
+                  sn)))
+            with (equivocators_state_project eqv_choice s)
+            ; try assumption.
+          apply functional_extensionality_dep.
+          intros [eqv'|neqv']; unfold equivocators_state_project.
+          ** destruct (eqv_choice eqv') eqn:Heqv'; try reflexivity.
+            destruct (decide (inl eqv' = inl ieqv)).
+            --- inversion e. subst.
+              rewrite state_update_eq.
+              unfold equivocator_state_extend.
+              rewrite Hsieqv.
+              specialize (Heqvs ieqv).
+              rewrite Heqv' in Heqvs. simpl in Heqvs.
+              rewrite Hsieqv in Heqvs. simpl in Heqvs.
+              destruct (le_lt_dec (S n) n0). { lia. }
+              destruct (le_lt_dec (S (S n)) n0). { lia. }
+              rewrite to_nat_of_nat.
+              destruct (nat_eq_dec n0 (S n)). { lia. }
+              f_equal. apply of_nat_ext.
+            --- rewrite state_update_neq; try assumption. reflexivity.
+          ** rewrite state_update_neq; try reflexivity.
+            intro contra. discriminate contra.
+        ++ specialize (Heqv ieqv) as Heqvi. unfold proper_descriptor in Heqvi.
+          rewrite Hieqv in Heqvi. rewrite state_update_eq in Heqvi.
+          simpl in Heqvi.
+          destruct (nat_eq_dec iieqv (S n)).
+          ** subst.
+            pose (equivocators_choice_update eqv_choice ieqv (NewMachine _ sn)) as eqv_choice'.
+            specialize (IHHes1 eqv_choice').
+            spec IHHes1.
+            { intro eqv'. spec Heqv eqv'.
+              destruct (decide (inl eqv' = inl ieqv)).
+              - inversion e. subst.
+                unfold eqv_choice'.
+                rewrite equivocators_choice_update_eq.
+                assumption.
+              - rewrite state_update_neq in Heqv; try assumption.
+                unfold eqv_choice'.
+                assert (n' : eqv' <> ieqv) by (intro contra; subst; elim n0; reflexivity).
+                rewrite equivocators_choice_update_neq; assumption.
+            }
+            replace
+              (equivocators_state_project eqv_choice
+              (state_update equivocator_IM s (inl ieqv)
+                 (equivocator_state_extend (IM (inl ieqv))
+                    (existT (fun n0 : nat => t (S n0) -> vstate (IM (inl ieqv))) n bs)
+                    sn)))
+              with
+                (equivocators_state_project eqv_choice' s)
+            ; try assumption.
+            apply functional_extensionality_dep.
+            intro i.
+            unfold equivocators_state_project at 1. unfold eqv_choice'.
+            rewrite equivocators_state_project_state_update_eqv.
+            destruct (decide (i = inl ieqv)).
+            --- subst. repeat rewrite state_update_eq.
+              rewrite equivocators_choice_update_eq.
+              rewrite Hieqv. unfold equivocator_state_extend.
+              unfold projT1. unfold projT2.
+              destruct (le_lt_dec (S (S n)) (S n)). { lia. }
+              rewrite to_nat_of_nat.
+              destruct (nat_eq_dec (S n) (S n)); congruence.
+            --- repeat rewrite state_update_neq; try assumption.
+              unfold equivocators_state_project.
+              destruct i; try reflexivity.
+              rewrite equivocators_choice_update_neq ; congruence.
+          ** assert (Heqvs : proper_equivocators_choice eqv_choice s).
+            { intro eqv'. specialize (Heqv eqv').
+              simpl in *.
+              destruct (decide (inl eqv' = inl ieqv))
+              ; try (rewrite state_update_neq in Heqv; assumption).
+              inversion e. subst. rewrite state_update_eq in Heqv.
+              rewrite Hieqv in *. simpl in Heqv. simpl.
+              rewrite Hsieqv. simpl. lia.
+            }
+            specialize (IHHes1 _ Heqvs).
+            replace
+              (equivocators_state_project eqv_choice
+              (state_update equivocator_IM s (inl ieqv)
+                 (equivocator_state_extend (IM (inl ieqv))
+                    (existT (fun n0 : nat => t (S n0) -> vstate (IM (inl ieqv))) n bs)
+                    sn)))
+              with (equivocators_state_project eqv_choice s)
+              ; try assumption.
+            apply functional_extensionality_dep.
+            intros [eqv'|neqv']; unfold equivocators_state_project.
+            --- destruct (eqv_choice eqv') eqn:Heqv'; try reflexivity.
+              destruct (decide (inl eqv' = inl ieqv)).
+              +++ inversion e. subst.
+                rewrite state_update_eq.
+                unfold equivocator_state_extend.
+                rewrite Hsieqv.
+                specialize (Heqvs ieqv).
+                rewrite Heqv' in Heqvs. simpl in Heqvs.
+                rewrite Hsieqv in Heqvs. simpl in Heqvs.
+                destruct (le_lt_dec (S n) n1). { lia. }
+                destruct (le_lt_dec (S (S n)) n1). { lia. }
+                rewrite to_nat_of_nat.
+                destruct (nat_eq_dec n1 (S n)). { lia. }
+                f_equal. apply of_nat_ext.
+              +++ rewrite state_update_neq; try assumption. reflexivity.
+            --- rewrite state_update_neq; try reflexivity.
+              intro contra. discriminate contra.
+      -- destruct Hv as [Hi Hv].
+        destruct (le_lt_dec (S (projT1 (s (inl ieqv)))) i). { lia. }
+        unfold fst in Ht.
+        destruct (vtransition (IM (inl ieqv)) li (projT2 (s (inl ieqv)) (of_nat_lt l), om0))
+          as (sieqv', om0') eqn:Ht'.
+        destruct fi eqn:Hfi; inversion Ht; subst si' om'; clear Ht.
+        ++ pose
+          (equivocators_choice_update
+            (fun eqv => NewMachine _ (proj1_sig (vs0 (IM (inl eqv)))))
+            ieqv (Existing _ i false)
+          ) as eqv_choice'.
+          specialize (IHHes1 eqv_choice') as Hs_om'.
+          spec Hs_om'.
+          { intro eqv'. unfold eqv_choice'.
+            destruct (decide (eqv' = ieqv)).
+            + subst. rewrite equivocators_choice_update_eq. assumption.
+            + rewrite equivocators_choice_update_neq; try assumption.
+              simpl. destruct (vs0 (IM (inl eqv'))). assumption.
+          }
+          destruct Hs_om' as [_oms Hs_om'].
+          destruct IHHes2 as [_som0 Hom0].
+          specialize (Hgen_om' _ _ Hs_om' _ _ Hom0).
+          spec Hgen_om'.
+          { split; try exact I.
+            unfold free_composite_valid.
+            unfold equivocators_state_project.
+            unfold eqv_choice'.
+            rewrite equivocators_choice_update_eq.
+            destruct (s (inl ieqv)) as (nieqv, bsieqv).
+            simpl in Hi.
+            destruct (le_lt_dec (S nieqv) i). { lia. }
+            replace (of_nat_lt l0) with (of_nat_lt Hi); try apply of_nat_ext.
+            assumption.
+          }
+          remember (equivocators_state_project eqv_choice' s) as sp.
+          simpl in Hgen_om'.
+          subst sp. unfold equivocators_state_project at 1 in Hgen_om'.
+          unfold eqv_choice' at 1 in Hgen_om'.
+          rewrite equivocators_choice_update_eq in Hgen_om'.
+          destruct (s (inl ieqv)) as (nieqv, bsieqv) eqn:Hsieqv.
+          simpl in Hi.
+          destruct (le_lt_dec (S nieqv) i). { lia. }
+          simpl in l. simpl in Ht'.
+          replace (of_nat_lt l) with (of_nat_lt Hi) in * by apply of_nat_ext.
+          clear l.
+          replace (of_nat_lt l0) with (of_nat_lt Hi) in * by apply of_nat_ext.
+          clear l0.
+          rewrite Ht' in Hgen_om'.
+          split; try (eexists _; apply Hgen_om').
+          intros eqv_choice Heqv.
+          unfold_transition Hgen_om'.
+          destruct (eqv_choice ieqv) as [sieqv | iieqv fieqv] eqn:Hieqv.
+          ** assert (Heqvs : proper_equivocators_choice eqv_choice s).
+            { intro eqv'. specialize (Heqv eqv').
+              simpl in *.
+              destruct (decide (inl eqv' = inl ieqv))
+              ; try (rewrite state_update_neq in Heqv; assumption).
+              inversion e. subst. rewrite state_update_eq in Heqv.
+              rewrite Hieqv in *. simpl in Heqv. assumption.
+            }
+            specialize (IHHes1 _ Heqvs).
+            replace
+              (equivocators_state_project eqv_choice
+              (state_update equivocator_IM s (inl ieqv)
+                 (equivocator_state_extend (IM (inl ieqv))
+                    (existT (fun n : nat => t (S n) -> vstate (IM (inl ieqv))) nieqv bsieqv) sieqv')))
+              with (equivocators_state_project eqv_choice s)
+              ; try assumption.
+            apply functional_extensionality_dep.
+            intros [eqv'|neqv']; unfold equivocators_state_project.
+            --- destruct (eqv_choice eqv') eqn:Heqv'; try reflexivity.
+              destruct (decide (inl eqv' = inl ieqv)).
+              +++ inversion e. subst.
+                rewrite state_update_eq.
+                unfold equivocator_state_extend.
+                rewrite Hsieqv.
+                specialize (Heqvs ieqv).
+                rewrite Heqv' in Heqvs. simpl in Heqvs.
+                rewrite Hsieqv in Heqvs. simpl in Heqvs.
+                destruct (le_lt_dec (S nieqv) n). { lia. }
+                destruct (le_lt_dec (S (S nieqv)) n). { lia. }
+                rewrite to_nat_of_nat.
+                destruct (nat_eq_dec n (S nieqv)). { lia. }
+                f_equal. apply of_nat_ext.
+              +++ rewrite state_update_neq; try assumption. reflexivity.
+            --- rewrite state_update_neq; try reflexivity.
+              intro contra. discriminate contra.
+          ** specialize (Heqv ieqv) as Heqvi. unfold proper_descriptor in Heqvi.
+            rewrite Hieqv in Heqvi. rewrite state_update_eq in Heqvi.
+            simpl in Heqvi.
+            destruct (nat_eq_dec iieqv (S nieqv)).
+            --- subst.
+              pose (equivocators_choice_update eqv_choice ieqv (Existing _ i false)) as eqv_choice''.
+              specialize (IHHes1 eqv_choice'').
+              spec IHHes1.
+              { intro eqv'. spec Heqv eqv'.
+                destruct (decide (inl eqv' = inl ieqv)).
+                - inversion e. subst.
+                  unfold eqv_choice''.
+                  rewrite equivocators_choice_update_eq.
+                  simpl. rewrite Hsieqv.
+                  assumption.
+                - rewrite state_update_neq in Heqv; try assumption.
+                  unfold eqv_choice''.
+                  assert (n' : eqv' <> ieqv) by (intro contra; subst; elim n; reflexivity).
+                  rewrite equivocators_choice_update_neq; assumption.
+              }
+              specialize (Hgen (existT _ (inl ieqv) li)).
+              destruct IHHes1 as [_oms' Hs].
+              specialize (Hgen _ _ Hs _ _ Hom0).
+              spec Hgen.
+              { split; try exact I.
+                unfold free_composite_valid. unfold vvalid. simpl in Hv.
+                replace (equivocators_state_project eqv_choice'' s (inl ieqv)) with (bsieqv (of_nat_lt Hi)); try assumption.
+                unfold eqv_choice''.
+                unfold equivocators_state_project.
+                rewrite equivocators_choice_update_eq.
+                rewrite Hsieqv.
+                destruct (le_lt_dec (S nieqv) i). { lia. }
+                f_equal. apply of_nat_ext.
+              }
+              unfold transition in Hgen.
+              unfold X in Hgen at 2. unfold free_composite_vlsm in Hgen.
+              unfold composite_vlsm in Hgen.
+              unfold mk_vlsm in Hgen.
+              unfold machine in Hgen.
+              unfold projT2 in Hgen.
+              unfold composite_vlsm_machine in Hgen.
+              unfold composite_transition in Hgen.
+              unfold equivocators_state_project at 1 in Hgen.
+              unfold eqv_choice'' in Hgen.
+              rewrite equivocators_choice_update_eq in Hgen.
+              rewrite Hsieqv in Hgen.
+              destruct (le_lt_dec (S nieqv) i). { lia. }
+              replace (of_nat_lt l) with (of_nat_lt Hi) in * by apply of_nat_ext.
+              rewrite Ht' in Hgen.
+              exists om0'.
+              replace
+                (equivocators_state_project eqv_choice
+                (state_update equivocator_IM s (inl ieqv)
+                   (equivocator_state_extend (IM (inl ieqv))
+                      (existT (fun n : nat => t (S n) -> vstate (IM (inl ieqv))) nieqv bsieqv) sieqv')))
+                with (state_update IM
+                (equivocators_state_project
+                   (equivocators_choice_update eqv_choice ieqv (Existing (IM (inl ieqv)) i false)) s)
+                (inl ieqv) sieqv')
+                ; try assumption.
+              apply functional_extensionality_dep.
+              intro i'.
+              rewrite equivocators_state_project_state_update_eqv.
+              destruct (decide (i' = inl ieqv)).
+              +++ subst. repeat rewrite state_update_eq.
+                rewrite Hieqv. unfold equivocator_state_extend.
+                unfold projT1. unfold projT2.
+                destruct (le_lt_dec (S (S nieqv)) (S nieqv)). { lia. }
+                rewrite to_nat_of_nat.
+                destruct (nat_eq_dec (S nieqv) (S nieqv)); try (elim n; reflexivity).
+                reflexivity.
+              +++ repeat rewrite state_update_neq; try assumption.
+                unfold equivocators_state_project.
+                destruct i'; try reflexivity.
+                rewrite equivocators_choice_update_neq
+                ; try (intro contra; subst; elim n; reflexivity).
+                reflexivity.
+            --- assert (Heqvs : proper_equivocators_choice eqv_choice s).
+              { intro eqv'. specialize (Heqv eqv').
+                simpl in *.
+                destruct (decide (inl eqv' = inl ieqv))
+                ; try (rewrite state_update_neq in Heqv; assumption).
+                inversion e. subst. rewrite state_update_eq in Heqv.
+                rewrite Hieqv in *. simpl in Heqv. simpl.
+                rewrite Hsieqv. simpl. lia.
+              }
+              specialize (IHHes1 _ Heqvs).
+              replace
+                (equivocators_state_project eqv_choice
+                (state_update equivocator_IM s (inl ieqv)
+                   (equivocator_state_extend (IM (inl ieqv))
+                      (existT (fun n0 : nat => t (S n0) -> vstate (IM (inl ieqv))) nieqv bsieqv) sieqv')))
+                with (equivocators_state_project eqv_choice s)
+                ; try assumption.
+              apply functional_extensionality_dep.
+              intros [eqv'|neqv']; unfold equivocators_state_project.
+              +++ destruct (eqv_choice eqv') eqn:Heqv'; try reflexivity.
+                destruct (decide (inl eqv' = inl ieqv)).
+                *** inversion e. subst.
+                  rewrite state_update_eq.
+                  unfold equivocator_state_extend.
+                  rewrite Hsieqv.
+                  specialize (Heqvs ieqv).
+                  rewrite Heqv' in Heqvs. simpl in Heqvs.
+                  rewrite Hsieqv in Heqvs. simpl in Heqvs.
+                  destruct (le_lt_dec (S nieqv) n0). { lia. }
+                  destruct (le_lt_dec (S (S nieqv)) n0). { lia. }
+                  rewrite to_nat_of_nat.
+                  destruct (nat_eq_dec n0 (S nieqv)). { lia. }
+                  f_equal. apply of_nat_ext.
+                *** rewrite state_update_neq; try assumption. reflexivity.
+              +++ rewrite state_update_neq; try reflexivity.
+                intro contra. discriminate contra.
+        ++ pose
+          (equivocators_choice_update
+            (fun eqv => NewMachine _ (proj1_sig (vs0 (IM (inl eqv)))))
+            ieqv (Existing _ i false)
+          ) as eqv_choice'.
+          specialize (IHHes1 eqv_choice') as Hs_om'.
+          spec Hs_om'.
+          { intro eqv'. unfold eqv_choice'.
+            destruct (decide (eqv' = ieqv)).
+            + subst. rewrite equivocators_choice_update_eq. assumption.
+            + rewrite equivocators_choice_update_neq; try assumption.
+              simpl. destruct (vs0 (IM (inl eqv'))). assumption.
+          }
+          destruct Hs_om' as [_oms Hs_om'].
+          destruct IHHes2 as [_som0 Hom0].
+          specialize (Hgen_om' _ _ Hs_om' _ _ Hom0).
+          spec Hgen_om'.
+          { split; try exact I.
+            unfold free_composite_valid.
+            unfold equivocators_state_project.
+            unfold eqv_choice'.
+            rewrite equivocators_choice_update_eq.
+            destruct (s (inl ieqv)) as (nieqv, bsieqv).
+            simpl in Hi.
+            destruct (le_lt_dec (S nieqv) i). { lia. }
+            replace (of_nat_lt l0) with (of_nat_lt Hi); try apply of_nat_ext.
+            assumption.
+          }
+          remember (equivocators_state_project eqv_choice' s) as sp.
+          simpl in Hgen_om'.
+          subst sp. unfold equivocators_state_project at 1 in Hgen_om'.
+          unfold eqv_choice' at 1 in Hgen_om'.
+          rewrite equivocators_choice_update_eq in Hgen_om'.
+          destruct (s (inl ieqv)) as (nieqv, bsieqv) eqn:Hsieqv.
+          simpl in Hi.
+          destruct (le_lt_dec (S nieqv) i). { lia. }
+          simpl in Ht'.
+          replace (of_nat_lt l0) with (of_nat_lt Hi) in * by apply of_nat_ext.
+          clear l0.
+          simpl in l.
+          replace (of_nat_lt l) with (of_nat_lt Hi) in * by apply of_nat_ext.
+          rewrite Ht' in Hgen_om'.
+          split; try (eexists _; apply Hgen_om').
+          intros eqv_choice Heqv.
+          destruct (eqv_choice ieqv) as [sieqv | iieqv fieqv] eqn:Hieqv.
+          ** assert (Heqvs : proper_equivocators_choice eqv_choice s).
+            { intro eqv'. specialize (Heqv eqv').
+              simpl in *.
+              destruct (decide (inl eqv' = inl ieqv))
+              ; try (rewrite state_update_neq in Heqv; assumption).
+              inversion e. subst. rewrite state_update_eq in Heqv.
+              rewrite Hieqv in *. simpl in Heqv. assumption.
+            }
+            specialize (IHHes1 _ Heqvs).
+            replace
+              (equivocators_state_project eqv_choice
+              (state_update equivocator_IM s (inl ieqv)
+                 (equivocator_state_update (IM (inl ieqv))
+                    (existT (fun n : nat => t (S n) -> vstate (IM (inl ieqv))) nieqv bsieqv)
+                    (of_nat_lt l) sieqv')))
+              with (equivocators_state_project eqv_choice s)
+              ; try assumption.
+            apply functional_extensionality_dep.
+            intros [eqv'|neqv']; unfold equivocators_state_project.
+            --- destruct (eqv_choice eqv') eqn:Heqv'; try reflexivity.
+              destruct (decide (inl eqv' = inl ieqv)).
+              +++ inversion e. subst.
+                rewrite Hieqv in Heqv'. discriminate Heqv'.
+              +++ rewrite state_update_neq; try assumption. reflexivity.
+            --- rewrite state_update_neq; try reflexivity.
+              intro contra. discriminate contra.
+          ** specialize (Heqv ieqv) as Heqvi. unfold proper_descriptor in Heqvi.
+            rewrite Hieqv in Heqvi. rewrite state_update_eq in Heqvi.
+            simpl in Heqvi.
+            destruct (nat_eq_dec iieqv i).
+            --- subst.
+              pose (equivocators_choice_update eqv_choice ieqv (Existing _ i false)) as eqv_choice''.
+              specialize (IHHes1 eqv_choice'').
+              spec IHHes1.
+              { intro eqv'. spec Heqv eqv'.
+                destruct (decide (inl eqv' = inl ieqv)).
+                - inversion e. subst.
+                  unfold eqv_choice''.
+                  rewrite equivocators_choice_update_eq.
+                  simpl. rewrite Hsieqv.
+                  assumption.
+                - rewrite state_update_neq in Heqv; try assumption.
+                  unfold eqv_choice''.
+                  assert (n' : eqv' <> ieqv) by (intro contra; subst; elim n; reflexivity).
+                  rewrite equivocators_choice_update_neq; assumption.
+              }
+              specialize (Hgen (existT _ (inl ieqv) li)).
+              destruct IHHes1 as [_oms' Hs].
+              specialize (Hgen _ _ Hs _ _ Hom0).
+              spec Hgen.
+              { split; try exact I.
+                unfold free_composite_valid. unfold vvalid. simpl in Hv.
+                replace (equivocators_state_project eqv_choice'' s (inl ieqv)) with (bsieqv (of_nat_lt Hi)); try assumption.
+                unfold eqv_choice''.
+                unfold equivocators_state_project.
+                rewrite equivocators_choice_update_eq.
+                rewrite Hsieqv.
+                destruct (le_lt_dec (S nieqv) i). { lia. }
+                f_equal. apply of_nat_ext.
+              }
+              unfold transition in Hgen.
+              unfold X in Hgen at 2. unfold free_composite_vlsm in Hgen.
+              unfold composite_vlsm in Hgen.
+              unfold mk_vlsm in Hgen.
+              unfold machine in Hgen.
+              unfold projT2 in Hgen.
+              unfold composite_vlsm_machine in Hgen.
+              unfold composite_transition in Hgen.
+              unfold equivocators_state_project at 1 in Hgen.
+              unfold eqv_choice'' in Hgen.
+              rewrite equivocators_choice_update_eq in Hgen.
+              rewrite Hsieqv in Hgen.
+              destruct (le_lt_dec (S nieqv) i). { lia. }
+              replace (of_nat_lt l0) with (of_nat_lt Hi) in * by apply of_nat_ext.
+              rewrite Ht' in Hgen.
+              exists om0'.
+              replace
+                (equivocators_state_project eqv_choice
+                (state_update equivocator_IM s (inl ieqv)
+                   (equivocator_state_update (IM (inl ieqv))
+                      (existT (fun n : nat => t (S n) -> vstate (IM (inl ieqv))) nieqv bsieqv)
+                      (of_nat_lt l) sieqv')))
+                with (state_update IM
+                (equivocators_state_project
+                   (equivocators_choice_update eqv_choice ieqv (Existing (IM (inl ieqv)) i false)) s)
+                (inl ieqv) sieqv')
+                ; try assumption.
+              apply functional_extensionality_dep.
+              intro i'.
+              rewrite equivocators_state_project_state_update_eqv.
+              destruct (decide (i' = inl ieqv)).
+              +++ subst. repeat rewrite state_update_eq.
+                rewrite Hieqv. unfold equivocator_state_update at 1.
+                unfold projT1.
+                destruct (le_lt_dec (S nieqv) i). { lia. }
+                unfold equivocator_state_update. unfold projT2.
+                rewrite eq_dec_if_true; try reflexivity.
+                apply of_nat_ext.
+              +++ repeat rewrite state_update_neq; try assumption.
+                unfold equivocators_state_project.
+                destruct i'; try reflexivity.
+                rewrite equivocators_choice_update_neq
+                ; try (intro contra; subst; elim n; reflexivity).
+                reflexivity.
+            --- assert (Heqvs : proper_equivocators_choice eqv_choice s).
+              { intro eqv'. specialize (Heqv eqv').
+                simpl in *.
+                destruct (decide (inl eqv' = inl ieqv))
+                ; try (rewrite state_update_neq in Heqv; assumption).
+                inversion e. subst. rewrite state_update_eq in Heqv.
+                rewrite Hieqv in *. simpl in Heqv. simpl.
+                rewrite Hsieqv. simpl. lia.
+              }
+              specialize (IHHes1 _ Heqvs).
+              replace
+                (equivocators_state_project eqv_choice
+                (state_update equivocator_IM s (inl ieqv)
+                   (equivocator_state_update (IM (inl ieqv))
+                      (existT (fun n0 : nat => t (S n0) -> vstate (IM (inl ieqv))) nieqv bsieqv)
+                      (of_nat_lt l) sieqv')))
+                with (equivocators_state_project eqv_choice s)
+                ; try assumption.
+              apply functional_extensionality_dep.
+              intros [eqv'|neqv']; unfold equivocators_state_project.
+              +++ destruct (eqv_choice eqv') eqn:Heqv'; try reflexivity.
+                destruct (decide (inl eqv' = inl ieqv)).
+                *** inversion e. subst.
+                  rewrite state_update_eq.
+                  unfold equivocator_state_extend.
+                  rewrite Hsieqv.
+                  specialize (Heqvs ieqv).
+                  rewrite Heqv' in Heqvs. simpl in Heqvs.
+                  rewrite Hsieqv in Heqvs. simpl in Heqvs.
+                  destruct (le_lt_dec (S nieqv) n0). { lia. }
+                  destruct (le_lt_dec (S (S nieqv)) n0). { lia. }
+                  unfold equivocator_state_update.
+                  unfold projT1.
+                  destruct (le_lt_dec (S nieqv) n0). { lia. }
+                  rewrite Hieqv in Heqv'.
+                  inversion Heqv'. subst n0 b. clear Heqv'.
+                  unfold projT2.
+                  rewrite eq_dec_if_false; try (f_equal; apply of_nat_ext).
+                  intro contra. elim n.
+                  apply (f_equal to_nat) in contra.
+                  repeat rewrite to_nat_of_nat in contra.
+                  inversion contra. reflexivity.
+                *** rewrite state_update_neq; try assumption. reflexivity.
+              +++ rewrite state_update_neq; try reflexivity.
+                intro contra. discriminate contra.
+    * specialize (Hgen (existT _ (inr ineqv) li)).
+      unfold vvalid in Hv. simpl in Hv.
+      unfold vtransition in Ht. simpl in Ht.
+      pose (fun eqv => NewMachine _ (proj1_sig (vs0 (IM (inl eqv))))) as eqv_choice.
+      specialize (IHHes1 eqv_choice) as Hs_om'.
+      spec Hs_om'.
+      { intro eqv'. unfold eqv_choice.
+        simpl. destruct (vs0 (IM (inl eqv'))). assumption.
+      }
+      destruct Hs_om' as [_oms Hs_om'].
+      destruct IHHes2 as [_som0 Hom0].
+      specialize (Hgen _ _ Hs_om' _ _ Hom0) as Hgen_om'.
+      spec Hgen_om'. { split; try exact I. assumption. }
+      remember (equivocators_state_project eqv_choice s) as sp.
+      simpl in Hgen_om'.
+      unfold vtransition in Hgen_om'.
+      subst sp. unfold equivocators_state_project at 1 in Hgen_om'.
+      rewrite Ht in Hgen_om'.
+      split; try (eexists _; apply Hgen_om').
+      clear eqv_choice Hgen_om' Hs_om'.
+      intros eqv_choice Heqv.
+      assert (Heqvs : proper_equivocators_choice eqv_choice s).
+      { intro eqv'. specialize (Heqv eqv').
+        rewrite state_update_neq in Heqv; congruence.
+      }
+      specialize (IHHes1 _ Heqvs).
+      destruct IHHes1 as [_oms' Hs].
+      specialize (Hgen _ _ Hs _ _ Hom0).
+      spec Hgen. { split; try exact I. assumption. }
+      unfold transition in Hgen.
+      unfold X in Hgen at 2. unfold free_composite_vlsm in Hgen.
+      unfold composite_vlsm in Hgen.
+      unfold mk_vlsm in Hgen.
+      unfold machine in Hgen.
+      unfold projT2 in Hgen.
+      unfold composite_vlsm_machine in Hgen.
+      unfold composite_transition in Hgen.
+      unfold equivocators_state_project at 1 in Hgen.
+      unfold vtransition in Hgen. rewrite Ht in Hgen.
+      exists om'.
+      rewrite equivocators_state_project_state_update_neqv.
+      assumption.
+Qed.
+
+End fully_equivocating_composition.
